\newcommand{\propconstant}[1]{
  \begin{equation*}
      \gamma = \sqrt{(R + j\omega L)(G + j \omega C)} #1
  \end{equation*}
}

\newcommand{\propconstantnoloss}[1]{
  \begin{equation*}
      \gamma =j\omega \sqrt{ L C} #1
  \end{equation*}
}

\newcommand{\impedance}[1]{
  \begin{equation*}
      Z_0 = \sqrt{\frac{(R + j\omega L)}{(G + j \omega C)}}  #1
  \end{equation*}
}

\newcommand{\impedancenoloss}[1]{
  \begin{equation*}
    Z_0 = \sqrt{\frac{L}{C}} #1
  \end{equation*}
}

\newcommand{\swr}[1]{
  \begin{equation*}
    SWR = \frac{1 + | \Gamma_L |}{1 - | \Gamma_L |} #1
  \end{equation*}

}
